revert of removal of tsl_error + use global_context instead of ad-hoc get_ind

translations/translation_utils.v
@@ -22,13 +22,46 @@ Definition tsl_context := (global_context * tsl_table)%type.
 
 Definition emptyTC : tsl_context := ([], []).
 
+Inductive tsl_error :=
+| NotEnoughFuel
+| TranslationNotFound (id : ident)
+| TranslationNotHandeled
+| TypingError (t : type_error).
+
+Inductive tsl_result A :=
+| Success : A -> tsl_result A
+| Error : tsl_error -> tsl_result A.
+
+Arguments Success {_} _.
+Arguments Error {_} _.
+
+Instance tsl_monad : Monad tsl_result :=
+  {| ret A a := Success a ;
+     bind A B m f :=
+       match m with
+       | Success a => f a
+       | Error e => Error e
+       end
+  |}.
+
+Instance monad_exc : MonadExc tsl_error tsl_result :=
+  { raise A e := Error e;
+    catch A m f :=
+      match m with
+      | Success a => m
+      | Error t => f t
+      end
+  }.
+
+
 
 Class Translation := { tsl_id : ident -> ident ;
-                       tsl_tm : tsl_context -> term -> TemplateMonad term ;
-                       tsl_ty : tsl_context -> term -> TemplateMonad term ;
+                       tsl_tm : tsl_context -> term -> tsl_result term ;
+                       tsl_ty : tsl_context -> term -> tsl_result term ;
                        tsl_ind : tsl_context -> kername -> kername -> minductive_decl
-                            -> TemplateMonad (tsl_table * list minductive_decl)
+                            -> tsl_result (tsl_table * list minductive_decl)
                      }.
+
 
 Definition tsl_ident (id : ident) : ident := (id ++ "ᵗ")%string.
 
@@ -37,6 +70,7 @@ Definition tsl_name tsl_ident n :=
   | nAnon => nAnon
   | nNamed n => nNamed (tsl_ident n)
   end.
+
 
 
 Definition tTranslate {tsl : Translation} (ΣE : tsl_context) (id : ident)
@@ -50,49 +84,61 @@ Definition tTranslate {tsl : Translation} (ΣE : tsl_context) (id : ident)
   | Some (ConstructRef (mkInd kn n) _)
   | Some (IndRef (mkInd kn n)) =>
       d <- tmQuoteInductive id ;;
-      Edecls <- tmEval lazy (tsl_ind ΣE kn kn' d) ;; Edecls <- Edecls;; (*join*)
-      let (E, decls) := (Edecls : tsl_table * list minductive_decl) in
-      monad_fold_left (fun _ e => tmMkInductive' e) decls tt ;;
-      print_nf  (id ++ " has been translated as " ++ id') ;;
-      ret (InductiveDecl kn d :: fst ΣE, E ++ snd ΣE)%list
+      d' <- tmEval lazy (tsl_ind ΣE kn kn' d) ;;
+      match d' with
+      | Error e => print_nf e ;; fail_nf ("Translation error during the translation of the inductive " ++ id)
+      | Success (E, decls) =>
+        monad_fold_left (fun _ e => tmMkInductive' e) decls tt ;;
+        print_nf  (id ++ " has been translated as " ++ id') ;;
+        ret (InductiveDecl kn d :: fst ΣE, E ++ snd ΣE)%list
+      end
 
-  | Some (ConstRef kn) => 
+  | Some (ConstRef kn) =>
     e <- tmQuoteConstant kn true ;;
     match e with
     | ParameterEntry _ => fail_nf (id ++ "is an axiom, not a definition")
     | DefinitionEntry {| definition_entry_type := A;
                          definition_entry_body := t |} =>
-      t' <- tmEval lazy (tsl_tm ΣE t) ;; t' <- t' ;;
-      tmMkDefinition id' (t' : term) ;;
-      let decl := {| cst_universes := [];
-                     cst_type := A; cst_body := Some t |} in
-      let Σ' := ConstantDecl kn decl :: (fst ΣE) in
-      let E' := (ConstRef kn, tConst kn' []) :: (snd ΣE) in
-      print_nf  (id ++ " has been translated as " ++ id') ;;
-      ret (Σ', E')
+      t' <- tmEval lazy (tsl_tm ΣE t) ;;
+      match t' with
+      | Error e => print_nf e ;; fail_nf ("Translation error during the translation of the body of " ++ id)
+      | Success t' =>
+        tmMkDefinition id' t' ;;
+        let decl := {| cst_universes := [];
+                       cst_type := A; cst_body := Some t |} in
+        let Σ' := ConstantDecl kn decl :: (fst ΣE) in
+        let E' := (ConstRef kn, tConst kn' []) :: (snd ΣE) in
+        print_nf  (id ++ " has been translated as " ++ id') ;;
+        ret (Σ', E')
+      end
     end
   end.
+
 
 
 Definition tImplement {tsl : Translation} (ΣE : tsl_context)
            (id : ident) (A : Type)
   : TemplateMonad (tsl_context) :=
   tA <- tmQuote A ;;
-  tA' <- tmEval lazy (tsl_ty ΣE tA) ;; tA' <- tA' ;;
-  id' <- tmEval all (tsl_id id) ;;
-  A' <- tmUnquoteTyped Type tA' ;;
-  tmLemma id' A' ;;
-  tmAxiom id A ;;
-  gr <- tmAbout id ;;
-  match gr with
-  | Some (ConstRef kn) =>
-    let decl := {| cst_universes := [];
-                   cst_type := tA; cst_body := None |} in
-    let Σ' := ConstantDecl kn decl :: (fst ΣE) in
-    let E' := (ConstRef kn, tConst id' []) :: (snd ΣE) in
-    print_nf (id ++ " has been translated as " ++ id') ;;
-    ret (Σ', E')
-  | _ => fail_nf (id ++ " was not found or is not a constant, this is a bug")
+  tA' <- tmEval lazy (tsl_ty ΣE tA) ;;
+  match tA' with
+  | Error e => print_nf e ;; fail_nf ("Translation error during the translation of the type of " ++ id)
+  | Success tA' =>
+      id' <- tmEval all (tsl_id id) ;;
+      A' <- tmUnquoteTyped Type tA' ;;
+      tmLemma id' A' ;;
+      tmAxiom id A ;;
+      gr <- tmAbout id ;;
+      match gr with
+      | Some (ConstRef kn) =>
+        let decl := {| cst_universes := [];
+                       cst_type := tA; cst_body := None |} in
+        let Σ' := ConstantDecl kn decl :: (fst ΣE) in
+        let E' := (ConstRef kn, tConst id' []) :: (snd ΣE) in
+        print_nf (id ++ " has been translated as " ++ id') ;;
+        ret (Σ', E')
+      | _ => fail_nf (id ++ " was not found or is not a constant, this is a bug")
+      end
   end.
 
 
