translations/tsl_param3.v
@@ -40,19 +40,22 @@ Definition dummy_inductive_body function_name :=
   mkinductive_body (function_name ++ ": wrong inductive") (tRel 0) [] [] [].
 Definition dummy_minductive_decl := Build_minductive_decl 0 [].
 
-Fixpoint trivial_match (get_ind : kername -> minductive_decl)
-         (rarg : nat) (ty : term) (ter : term) : term :=
+Fixpoint trivial_match (Σ : global_context) (rarg : nat) (ty : term) (ter : term) : term :=
   match rarg, ty with
   | 0, tProd na A B => let (cind, args) := unapp B in
     match cind with
     | tInd (mkInd indname indnum) _ =>
-      let (p, bodys) := get_ind indname in
-      let body := nth indnum bodys (dummy_inductive_body "trivial_match") in
-      mkApps ttodo [ty]
+      match lookup_env Σ indname with
+      | Some (InductiveDecl _ (Build_minductive_decl p bodies)) =>
+        let body := nth indnum bodies (dummy_inductive_body "trivial_match") in
+        mkApps ttodo [ty]
+      | _ => debug_term ("trivial_match: inductive " ++ indname ++
+                         "not in global context")
+      end
     | _ => debug_term "trivial_match: not an inductive"
     end
   | S n, tProd na A B =>
-    tLambda nAnon A (trivial_match get_ind n B (lift 1 1 ter))
+    tLambda nAnon A (trivial_match Σ n B (lift 1 1 ter))
   | _, _ => debug_term "trivial_match: not enough products"
   end.
 
@@ -82,18 +85,18 @@ Fixpoint regroup (n : nat) k (t : term) : term :=
   end.
 Notation regroup0 n := (regroup n 0).
 
-Fixpoint tsl_rec1_app get_ind (app : option term) (E : tsl_table) (t : term) : term :=
-  let tsl_rec1_app := tsl_rec1_app get_ind in
+Fixpoint tsl_rec1_app (app : option term) (ΣE : tsl_context) (t : term) : term :=
+  let (Σ, E) := ΣE in
   let tsl_rec1 := tsl_rec1_app None in
   let debug case symbol :=
       debug_term ("tsl_rec1: " ++ case ++ " " ++ symbol ++ " not found") in
   match t with
   | tLambda na A t =>
     let A0 := tsl_rec0 0 A in
-    let A1 := tsl_rec1_app None E A in
+    let A1 := tsl_rec1_app None ΣE A in
     tLambda na A0 (tLambda (tsl_name tsl_ident na)
                            (subst_app (lift0 1 A1) [tRel 0])
-                           (tsl_rec1_app (option_map (lift 2 2) app) E t))
+                           (tsl_rec1_app (option_map (lift 2 2) app) ΣE t))
   | t => let t1 :=
   match t with
   | tRel k => tRel (2 * k)
@@ -101,9 +104,9 @@ Fixpoint tsl_rec1_app get_ind (app : option term) (E : tsl_table) (t : term) : t
 
   | tProd na A B =>
     let A0 := tsl_rec0 0 A in
-    let A1 := tsl_rec1 E A in
+    let A1 := tsl_rec1 ΣE A in
     let B0 := tsl_rec0 1 B in
-    let B1 := tsl_rec1 E B in
+    let B1 := tsl_rec1 ΣE B in
     let ΠAB0 := tProd na A0 B0 in
     tLambda (nNamed "f") ΠAB0
       (tProd na (lift0 1 A0)
@@ -112,23 +115,23 @@ Fixpoint tsl_rec1_app get_ind (app : option term) (E : tsl_table) (t : term) : t
                     (subst_app (lift 1 2 B1)
                                [tApp (tRel 2) [tRel 1]])))
   | tApp t us =>
-    let us' := concat (map (fun v => [tsl_rec0 0 v; tsl_rec1 E v]) us) in
-    mkApps (tsl_rec1 E t) us'
+    let us' := concat (map (fun v => [tsl_rec0 0 v; tsl_rec1 ΣE v]) us) in
+    mkApps (tsl_rec1 ΣE t) us'
 
   | tLetIn na t A u =>
     let t0 := tsl_rec0 0 t in
-    let t1 := tsl_rec1 E t in
+    let t1 := tsl_rec1 ΣE t in
     let A0 := tsl_rec0 0 A in
-    let A1 := tsl_rec1 E A in
+    let A1 := tsl_rec1 ΣE A in
     let u0 := tsl_rec0 0 u in
-    let u1 := tsl_rec1 E u in
+    let u1 := tsl_rec1 ΣE u in
     tLetIn na t0 A0 (tLetIn (tsl_name tsl_ident na) (lift0 1 t1)
                             (subst_app (lift0 1 A1) [tRel 0]) u1)
 
   | tCast t c A => let t0 := tsl_rec0 0 t in
-                  let t1 := tsl_rec1 E t in
+                  let t1 := tsl_rec1 ΣE t in
                   let A0 := tsl_rec0 0 A in
-                  let A1 := tsl_rec1 E A in
+                  let A1 := tsl_rec1 ΣE A in
                   tCast t1 c (mkApps A1 [tCast t0 c A0]) (* apply_subst ? *)
 
   | tConst s univs =>
@@ -152,19 +155,19 @@ Fixpoint tsl_rec1_app get_ind (app : option term) (E : tsl_table) (t : term) : t
     match lookup_tsl_table E (IndRef (fst ik)) with
     | Some (tInd i _univ) =>
       tCase (i, (snd ik) * 2)
-            (tsl_rec1_app (Some (tsl_rec0 0 case1)) E t)
-            (tsl_rec1 E u)
-            (map (on_snd (tsl_rec1 E)) brs)
+            (tsl_rec1_app (Some (tsl_rec0 0 case1)) ΣE t)
+            (tsl_rec1 ΣE u)
+            (map (on_snd (tsl_rec1 ΣE)) brs)
     | _ => debug "tCase" (match (fst ik) with mkInd s _ => s end)
     end
   | tFix fs k =>
     let N := List.length fs in
     let fs0 := map (map_def (tsl_rec0 0)) fs in
     let fs1 := map (fun dt =>
-      let rai := 2 * dt.(rarg) + 1 in let tyi := (tsl_rec1 E dt.(dtype)) in
+      let rai := 2 * dt.(rarg) + 1 in let tyi := (tsl_rec1 ΣE dt.(dtype)) in
       mkdef _ (tsl_name tsl_ident dt.(dname)) tyi
-         (tLetIn (nNamed "modfix") tyi (tsl_rec1 E dt.(dbody))
-                 (trivial_match get_ind rai (lift0 1 tyi) (tRel 0)))
+         (tLetIn (nNamed "modfix") tyi (tsl_rec1 ΣE dt.(dbody))
+                 (trivial_match Σ rai (lift0 1 tyi) (tRel 0)))
          rai) fs in
     fold_left_i (fun term i f0 => tLetIn (nNamed ("fix" ++ string_of_int k))
                 (nth k fs0 f0).(dtype) (tFix fs0 i) term) (rev fs0)
@@ -179,9 +182,9 @@ Fixpoint tsl_rec1_app get_ind (app : option term) (E : tsl_table) (t : term) : t
   match app with Some t' => mkApp t1 (t' {3 := tRel 1} {2 := tRel 0})
                | None => t1 end
   end.
-Definition tsl_rec1_ get_ind := tsl_rec1_app get_ind None.
+Definition tsl_rec1 := tsl_rec1_app None.
 
-Definition tsl_mind_decl_ (get_ind : kername -> minductive_decl) (E : tsl_table)
+Definition tsl_mind_decl (ΣE : tsl_context)
            (kn kn' : kername) (mind : minductive_decl) : tsl_table * list minductive_decl.
   refine (_, [{| ind_npars := 2 * mind.(ind_npars); ind_bodies := _ |}]).
   - refine (fold_left_i (fun E i ind => _ :: _ ++ E)%list mind.(ind_bodies) []).
@@ -198,7 +201,7 @@ Definition tsl_mind_decl_ (get_ind : kername -> minductive_decl) (E : tsl_table)
               ind_ctors := _;
               ind_projs := [] |}. (* todo *)
     + (* arity  *)
-      refine (let ar := subst_app (tsl_rec1_ get_ind E ind.(ind_type))
+      refine (let ar := subst_app (tsl_rec1 ΣE ind.(ind_type))
                                   [tInd (mkInd kn i) []] in
               ar).
     + (* constructors *)
@@ -206,59 +209,19 @@ Definition tsl_mind_decl_ (get_ind : kername -> minductive_decl) (E : tsl_table)
       intros k ((name, typ), nargs).
       refine (tsl_ident name, _, 2 * nargs).
       refine (subst_app _ [tConstruct (mkInd kn i) k []]).
-      refine (fold_left_i (fun t0 i u  => t0 {S i := u}) _ (tsl_rec1_ get_ind E typ)).
+      refine (fold_left_i (fun t0 i u  => t0 {S i := u}) _ (tsl_rec1 ΣE typ)).
       (* [I_n-1; ... I_0] *)
       refine (rev (map_i (fun i _ => tInd (mkInd kn i) [])
                               mind.(ind_bodies))).
 Defined.
 
-Definition swap_list_monad {M} {monadM : Monad M} {T} (l : list (M T)) : M (list T) :=
-  monad_fold_left (fun r mx => x <- mx;; ret (cons x r)) l [].
-Definition monad_concat {M} {monadM : Monad M} {T} (l : list (M (list T))) : M (list T) :=
-  l <- swap_list_monad l;; ret (concat l).
-Definition monad_map {T : Type -> Type} `{Monad T} {A B : Type} (f : A -> T B) (l : list A) : T (list B) :=
-  swap_list_monad (map f l).
-
-Definition tmQuoteInductivesOf (t : term) : TemplateMonad (kername -> minductive_decl) :=
-  let entry := (global_reference * minductive_decl)%type in
-  let monad_concat := @monad_concat TemplateMonad TemplateMonad_Monad entry in
-  let fix collect (t : term) : TemplateMonad (table minductive_decl) :=
-      match t with
-      | tInd (mkInd name _) _ =>  tmBind (tmQuoteInductive name) (fun decl =>
-                                  @tmReturn (list entry) [(ConstRef name, decl)])
-      | tEvar k ts => monad_concat (map collect ts)
-      | tCast t c a => monad_concat [collect t; collect a]
-      | tProd na A B => monad_concat [collect A; collect B]
-      | tLambda na A t => monad_concat [collect A; collect t]
-      | tLetIn na t A u => monad_concat [collect t; collect A; collect u]
-      | tApp t lu => monad_concat [collect t; monad_concat (map collect lu)]
-      | tCase ik t u br => monad_concat [collect t; collect u;
-                           monad_concat (map (fun x => collect (snd x)) br)]
-      | tProj p t => collect t
-      | tFix fs k | tCoFix fs k => monad_concat (map (fun df =>
-         monad_concat [collect df.(dtype); collect df.(dbody)]) fs)
-      | tRel _ | tVar _ | tMeta _ | tSort _ | tConst _ _ | tConstruct _ _ _ => tmReturn nil
-  end in
-  tmBind (collect t) (fun table =>
-  tmReturn (fun k => option_get dummy_minductive_decl (@lookup_table minductive_decl table (ConstRef k)))).
-
-Definition tsl_rec1 E t : TemplateMonad term :=
-  get_ind <- tmQuoteInductivesOf t;;
-  ret (tsl_rec1_ get_ind E t).
-
-Definition tsl_mind_decl (E : tsl_table) (kn kn' : kername) (mind : minductive_decl) :
-   TemplateMonad (tsl_table * list minductive_decl)%type :=
-   get_ind <- tmQuoteInductivesOf (tInd (mkInd kn 0) []);;
-   ret (tsl_mind_decl_ get_ind E kn kn' mind).
-
 
 Run TemplateProgram (tm <- tmQuote (forall A, A -> A) ;;
-                     get_ind <- tmQuoteInductivesOf tm;;
-                     tm' <- tsl_rec1 [] tm;;
+                     let tm' := tsl_rec1 ([],[]) tm in
                      tmUnquote tm' >>= tmPrint).
 
 Run TemplateProgram (tm <- tmQuote (fun A (x : A) => x) ;;
-                     tm' <- tsl_rec1 [] tm;;
+                     let tm' := tsl_rec1 ([],[]) tm in
                      tmUnquote tm' >>= tmPrint).
 
 Goal ((fun f : forall A : Type, A -> A =>
@@ -267,12 +230,13 @@ Goal ((fun f : forall A : Type, A -> A =>
 reflexivity.
 Defined.
 
-(* Breaks because tsl_result is not related to TemplateMonad *)
+
 Instance param : Translation :=
   {| tsl_id := tsl_ident ;
-     tsl_tm := fun ΣE t => tsl_rec1 (snd ΣE) t;
+     tsl_tm := fun ΣE t => ret (tsl_rec1 ΣE t) ;
      tsl_ty := fun '(Σ, E) t => todo "not meaningful here" ;
-     tsl_ind := fun ΣE kn kn' mind => tsl_mind_decl (snd ΣE) kn kn' mind |}.
+     tsl_ind := fun ΣE kn kn' mind => ret (tsl_mind_decl ΣE kn kn' mind) |}.
+
 
 Definition T := forall A, A -> A.
 Run TemplateProgram (tTranslate emptyTC "T").
